use Prop for typing judgment

theories/logrel_heaplang_sessions/ltyping.v
@@ -4,9 +4,11 @@ From iris.base_logic.lib Require Import invariants.
 From iris.heap_lang Require Import notation proofmode.
 
 (* The semantic typing judgment *)
+(* This is a Prop, which means that we cannot have typing judgments
+that are contingent on some resources being in the current context. *)
 Definition ltyped `{heapG Σ}
-    (Γ : gmap string (lty Σ)) (e : expr) (A : lty Σ) : iProp Σ :=
-  (□ ∀ vs, env_ltyped Γ vs -∗ WP subst_map vs e {{ A }})%I.
+    (Γ : gmap string (lty Σ)) (e : expr) (A : lty Σ) : Prop :=
+  ((∀ vs, env_ltyped Γ vs -∗ WP subst_map vs e {{ A }}) : iProp Σ)%I.
 
 Notation "Γ ⊨ e : A" := (ltyped Γ e A)
   (at level 100, e at next level, A at level 200).
