theories/logrel_heaplang_sessions/rules/mutex.v
@@ -25,7 +25,7 @@ Section properties.
   Lemma ltyped_mutexalloc A:
      ∅ ⊨ mutexalloc : A → mutex A.
   Proof.
-    iIntros (vs) "!> HΓ /=".
+    iIntros (vs) "HΓ /=".
     wp_apply wp_value.
     iIntros (v) "Hv".
     rewrite /mutexalloc. wp_pures.
@@ -44,7 +44,7 @@ Section properties.
   Lemma ltyped_mutexacquire A:
      ∅ ⊨ mutexacquire : mutex A → A * mutexguard A.
   Proof.
-    iIntros (vs) "!> HΓ /=".
+    iIntros (vs) "HΓ /=".
     wp_apply wp_value.
     iIntros (m) "Hm".
     iDestruct "Hm" as (N γ l lk ->) "#Hlock".
@@ -65,7 +65,7 @@ Section properties.
   Lemma ltyped_mutexrelease A:
     ∅ ⊨ mutexrelease : A → mutexguard A → mutex A.
   Proof.
-    iIntros (vs) "!> HΓ /=".
+    iIntros (vs) "HΓ /=".
     wp_apply wp_value.
     iIntros (w1) "Hw1".
     rewrite /mutexrelease. wp_pures.
