theories/logrel_heaplang_sessions/rules/rec.v
@@ -26,18 +26,20 @@ Section properties.
   Proof. apply fixpoint_unfold. Qed.
 
   Lemma ltyped_fold Γ e (B : ltyC Σ -n> ltyC Σ) :
-    (Γ ⊨ e : B (lty_rec B)) -∗ Γ ⊨ e : lty_rec B.
+    (Γ ⊨ e : B (lty_rec B)) → Γ ⊨ e : lty_rec B.
   Proof.
-    iIntros "#H" (vs) "!> HΓ /=".
-    wp_apply (wp_wand with "(H [HΓ //])"); iIntros (w) "HB".
+    intros He. iIntros (vs) "HΓ /=".
+    iPoseProof He as "He".
+    wp_apply (wp_wand with "(He [HΓ //])"); iIntros (w) "HB".
     by iEval (rewrite lty_rec_unfold /lty_car /=).
   Qed.
 
   Lemma ltyped_unfold Γ e (B : ltyC Σ -n> ltyC Σ) :
-    (Γ ⊨ e : lty_rec B) -∗ Γ ⊨ rec_unfold e : B (lty_rec B).
+    (Γ ⊨ e : lty_rec B) → Γ ⊨ rec_unfold e : B (lty_rec B).
   Proof.
-    iIntros "#H" (vs) "!> HΓ /=".
-    wp_apply (wp_wand with "(H [HΓ //])"); iIntros (w) "HB".
+    intros He. iIntros (vs) "HΓ /=".
+    iPoseProof He as "He".
+    wp_apply (wp_wand with "(He [HΓ //])"); iIntros (w) "HB".
     iEval (rewrite lty_rec_unfold /lty_car /=) in "HB". by wp_lam.
   Qed.
 End properties.
